src/phase2/weak_approx.lean
@@ -1,0 +1,288 @@
+import data.pfun
+import phase2.approximation
+import phase2.complete_orbit
+
+open cardinal set
+open_locale cardinal classical
+
+universe u
+
+namespace con_nf
+variable [params.{u}]
+
+/-!
+# Weak approximations
+-/
+
+/-- A *weak near-litter approximation* is a partial function from atoms to atoms and a partial
+function from litters to near-litters, both of which have small domain.
+The image of a litter under the `litter_map` should be interpreted as the intended *precise* image
+of this litter under an allowable permutation.
+The atom and litter maps should be injective (in suitable senses) and cohere in the sense that
+images of atoms in litters are mapped to atoms inside the corresponding near-litters. -/
+@[ext] structure weak_near_litter_approx :=
+(atom_map : atom →. atom)
+(litter_map : litter →. near_litter)
+(atom_map_dom_small : small atom_map.dom)
+(litter_map_dom_small : small litter_map.dom)
+(atom_map_injective : ∀ ⦃a b⦄ ha hb, (atom_map a).get ha = (atom_map b).get hb → a = b)
+(litter_map_injective : ∀ ⦃L₁ L₂ : litter⦄ hL₁ hL₂,
+  (((litter_map L₁).get hL₁ : set atom) ∩ (litter_map L₂).get hL₂).nonempty → L₁ = L₂)
+(atom_mem : ∀ (a : atom) ha L hL, a.1 = L ↔ (atom_map a).get ha ∈ (litter_map L).get hL)
+
+/-- A `β`-weak structural approximation is a product that assigns a weak near-litter approximation
+to each `β`-extended index. -/
+def weak_struct_approx (β : type_index) := extended_index β → weak_near_litter_approx
+
+namespace weak_near_litter_approx
+
+variable (w : weak_near_litter_approx)
+
+/-- A litter that is not allowed to be used as a sandbox because it appears somewhere that
+we need to preserve. -/
+@[mk_iff] inductive banned_litter : litter → Prop
+| atom_dom (a : atom) : (w.atom_map a).dom → banned_litter a.1
+| litter_dom (L : litter) : (w.litter_map L).dom → banned_litter L
+| atom_map (a : atom) (h) : banned_litter ((w.atom_map a).get h).1
+| litter_map (L : litter) (h) : banned_litter ((w.litter_map L).get h).1
+| diff (L : litter) (h) (a : atom) :
+    a ∈ ((w.litter_map L).get h : set atom) \ litter_set ((w.litter_map L).get h).1 →
+    banned_litter a.1
+
+/-- There are only a small amount of banned litters. -/
+lemma banned_litter_small : small {L | w.banned_litter L} :=
+begin
+  simp only [banned_litter_iff, mem_diff, set_like.mem_coe, mem_litter_set],
+  refine small.union _ (small.union _ (small.union _ (small.union _ _))),
+  { refine lt_of_le_of_lt _ w.atom_map_dom_small,
+    refine ⟨⟨λ a, ⟨_, a.prop.some_spec.1⟩, λ a₁ a₂ h, _⟩⟩,
+    simp only [subtype.mk_eq_mk, prod.mk.inj_iff] at h,
+    have := a₁.prop.some_spec.2,
+    rw h at this,
+    exact subtype.coe_injective (this.trans a₂.prop.some_spec.2.symm), },
+  { refine lt_of_le_of_lt _ w.litter_map_dom_small,
+    refine ⟨⟨λ L, ⟨_, L.prop⟩, λ L₁ L₂ h, _⟩⟩,
+    simp only [subtype.mk_eq_mk, prod.mk.inj_iff] at h,
+    exact subtype.coe_injective h, },
+  { refine lt_of_le_of_lt _ w.atom_map_dom_small,
+    refine ⟨⟨λ L, ⟨_, L.prop.some_spec.some⟩, λ L₁ L₂ h, _⟩⟩,
+    simp only [subtype.mk_eq_mk, prod.mk.inj_iff] at h,
+    have := L₁.prop.some_spec.some_spec,
+    simp_rw h at this,
+    exact subtype.coe_injective (this.trans L₂.prop.some_spec.some_spec.symm), },
+  { refine lt_of_le_of_lt _ w.litter_map_dom_small,
+    refine ⟨⟨λ L, ⟨_, L.prop.some_spec.some⟩, λ L₁ L₂ h, _⟩⟩,
+    simp only [subtype.mk_eq_mk, prod.mk.inj_iff] at h,
+    have := L₁.prop.some_spec.some_spec,
+    simp_rw h at this,
+    exact subtype.coe_injective (this.trans L₂.prop.some_spec.some_spec.symm), },
+  { have : small ⋃ (L : litter) (h : (w.litter_map L).dom),
+      ((w.litter_map L).get h : set atom) \ litter_set ((w.litter_map L).get h).1,
+    { refine small.bUnion _ _,
+      { refine lt_of_le_of_lt _ w.litter_map_dom_small,
+        refine ⟨⟨λ N, ⟨_, N.prop⟩, λ N₁ N₂ h, _⟩⟩,
+        simp only [subtype.mk_eq_mk, prod.mk.inj_iff] at h,
+        exact subtype.coe_inj.mp h, },
+      { intros L hL,
+        refine small.mono _ ((w.litter_map L).get hL).2.prop,
+        exact λ x hx, or.inr hx, }, },
+    refine lt_of_le_of_lt _ this,
+    refine ⟨⟨λ L, ⟨L.prop.some_spec.some_spec.some, _⟩, λ L₁ L₂ h, _⟩⟩,
+    { simp only [mem_Union],
+      exact ⟨_, _, L.prop.some_spec.some_spec.some_spec.1⟩, },
+    simp only [subtype.mk_eq_mk, prod.mk.inj_iff] at h,
+    have := L₁.prop.some_spec.some_spec.some_spec.2,
+    rw h at this,
+    exact subtype.coe_injective
+      (this.trans L₂.prop.some_spec.some_spec.some_spec.2.symm), },
+end
+
+lemma not_banned_litter_nonempty : nonempty {L | ¬w.banned_litter L} :=
+begin
+  rw ← mk_ne_zero_iff,
+  intro h,
+  have := mk_sum_compl {L | w.banned_litter L},
+  rw [compl_set_of, h, add_zero, mk_litter] at this,
+  exact κ_le_μ.not_lt (lt_of_eq_of_lt this.symm w.banned_litter_small),
+end
+
+/-- The *sandbox litter* for a weak near-litter approximation is an arbitrarily chosen litter that
+isn't banned. -/
+noncomputable def sandbox_litter : litter := w.not_banned_litter_nonempty.some
+
+lemma sandbox_litter_not_banned : ¬w.banned_litter w.sandbox_litter :=
+w.not_banned_litter_nonempty.some.prop
+
+/-- If `a` is in the domain, this is the atom map. Otherwise, this gives an arbitrary atom. -/
+noncomputable def atom_map_or_else (a : atom) : atom := (w.atom_map a).get_or_else (arbitrary atom)
+
+lemma atom_map_or_else_of_dom {a : atom} (ha : (w.atom_map a).dom) :
+  w.atom_map_or_else a = (w.atom_map a).get ha :=
+by rw [atom_map_or_else, part.get_or_else_of_dom]
+
+lemma mk_atom_map_image_le_mk_sandbox :
+  #(w.atom_map.dom ∆ (w.atom_map_or_else '' w.atom_map.dom) : set atom) ≤
+    #(litter_set w.sandbox_litter) :=
+begin
+  rw mk_litter_set,
+  refine le_trans (mk_subtype_mono symm_diff_subset_union) (le_trans (mk_union_le _ _) _),
+  refine add_le_of_le κ_regular.aleph_0_le _ _,
+  exact le_of_lt w.atom_map_dom_small,
+  exact le_trans mk_image_le (le_of_lt w.atom_map_dom_small),
+end
+
+lemma disjoint_sandbox :
+  disjoint (w.atom_map.dom ∪ w.atom_map_or_else '' w.atom_map.dom) (litter_set w.sandbox_litter) :=
+begin
+  rw [disjoint_iff_inter_eq_empty, eq_empty_iff_forall_not_mem],
+  rintros a ⟨ha₁, ha₂⟩,
+  rw mem_litter_set at ha₂,
+  have hnb := w.sandbox_litter_not_banned,
+  rw ← ha₂ at hnb,
+  cases ha₁,
+  { exact hnb (banned_litter.atom_dom a ha₁), },
+  { refine hnb _,
+    simp only [mem_image, pfun.mem_dom] at ha₁,
+    obtain ⟨b, ⟨_, hb, rfl⟩, rfl⟩ := ha₁,
+    rw w.atom_map_or_else_of_dom hb,
+    exact banned_litter.atom_map b hb, },
+end
+
+lemma atom_map_or_else_injective : inj_on w.atom_map_or_else w.atom_map.dom :=
+begin
+  intros a ha b hb h,
+  rw [w.atom_map_or_else_of_dom ha, w.atom_map_or_else_of_dom hb] at h,
+  exact w.atom_map_injective ha hb h,
+end
+
+/-- A local permutation induced by completing the orbits of atoms in a weak near-litter
+approximation. This function creates forward and backward images of atoms in the *sandbox litter*,
+a litter which is away from the domain and range of the approximation in question, so it should
+not interfere with other constructions. -/
+noncomputable def complete_atom_perm : local_perm atom :=
+local_perm.complete
+  w.atom_map_or_else
+  w.atom_map.dom
+  (litter_set w.sandbox_litter)
+  w.mk_atom_map_image_le_mk_sandbox
+  (by simpa only [mk_litter_set] using κ_regular.aleph_0_le)
+  w.disjoint_sandbox
+  w.atom_map_or_else_injective
+
+lemma sandbox_subset_small : small (local_perm.sandbox_subset
+  w.mk_atom_map_image_le_mk_sandbox
+  (by simpa only [mk_litter_set] using κ_regular.aleph_0_le)) :=
+begin
+  rw small,
+  rw cardinal.mk_congr (local_perm.sandbox_subset_equiv _ _),
+  simp only [mk_sum, mk_prod, mk_denumerable, lift_aleph_0, lift_uzero, lift_id],
+  refine add_lt_of_lt κ_regular.aleph_0_le _ _;
+    refine (mul_lt_of_lt κ_regular.aleph_0_le (lt_of_le_of_lt Λ_limit.aleph_0_le Λ_lt_κ) _);
+    refine lt_of_le_of_lt (mk_subtype_mono (diff_subset _ _)) _,
+  { exact w.atom_map_dom_small, },
+  { exact lt_of_le_of_lt mk_image_le w.atom_map_dom_small, },
+end
+
+lemma complete_atom_perm_domain_small : small w.complete_atom_perm.domain :=
+small.union (small.union w.atom_map_dom_small
+  (lt_of_le_of_lt mk_image_le w.atom_map_dom_small)) w.sandbox_subset_small
+
+/-- A near-litter approximation built from this weak near-litter approximation.
+Its action on atoms matches that of the weak approximation, and its rough action on litters
+matches the given litter permutation. -/
+noncomputable def complete (litter_perm : local_perm litter) : near_litter_approx := {
+  atom_perm := w.complete_atom_perm,
+  litter_perm := litter_perm,
+  domain_small := λ L, small.mono (inter_subset_right _ _) w.complete_atom_perm_domain_small,
+}
+
+variable {litter_perm : local_perm litter}
+
+lemma complete_atom_perm_apply_eq {a : atom} (ha : (w.atom_map a).dom) :
+  w.complete_atom_perm a = (w.atom_map a).get ha :=
+by rwa [complete_atom_perm, local_perm.complete_apply_eq, atom_map_or_else_of_dom]
+
+lemma complete_smul_atom_eq {a : atom} (ha : (w.atom_map a).dom) :
+  w.complete litter_perm • a = (w.atom_map a).get ha := w.complete_atom_perm_apply_eq ha
+
+@[simp] lemma complete_smul_litter_eq (L : litter) :
+  w.complete litter_perm • L = litter_perm L := rfl
+
+lemma smul_to_near_litter_eq_of_exactly_approximates
+  {π : near_litter_perm} (hπ : (w.complete litter_perm).exactly_approximates π)
+  {L : litter} (hL : (w.litter_map L).dom)
+  (hπL : π • L = ((w.litter_map L).get hL).1)
+  (hdiff : ((w.litter_map L).get hL : set atom) ∆
+    litter_set ((w.litter_map L).get hL).1 ⊆ w.atom_map.ran)
+  (hfwd : ∀ a ha, (w.atom_map a).get ha ∈ litter_set L → (w.atom_map ((w.atom_map a).get ha)).dom) :
+  π • L.to_near_litter = (w.litter_map L).get hL :=
+begin
+  refine set_like.coe_injective _,
+  ext a : 1,
+  simp only [mem_smul_set_iff_inv_smul_mem, near_litter_perm.coe_smul, litter.coe_to_near_litter,
+    mem_litter_set, set_like.mem_coe],
+  split,
+  { intro ha,
+    by_cases π.is_exception a,
+    { suffices h' : π⁻¹ • a ∈ w.atom_map.dom,
+      { rw w.atom_mem _ h' L hL at ha,
+        have := hπ.map_atom _ (or.inl (or.inl h')),
+        rw w.complete_smul_atom_eq h' at this,
+        rw [this, smul_inv_smul] at ha,
+        exact ha, },
+      rw ← hπ.symm_map_atom a (hπ.exception_mem _ h) at ha ⊢,
+      obtain ((hdom | hdom) | hdom) := (w.complete litter_perm).atom_perm.symm.map_domain
+        (hπ.exception_mem _ h),
+      { exact hdom, },
+      { obtain ⟨c, hc₁, hc₂⟩ := hdom,
+        rw w.atom_map_or_else_of_dom hc₁ at hc₂,
+        have := hfwd c hc₁ (by rwa hc₂),
+        rw hc₂ at this,
+        exact this, },
+      { cases w.sandbox_litter_not_banned _,
+        rw ← eq_of_mem_litter_set_of_mem_litter_set ha
+          (local_perm.sandbox_subset_subset _ _ hdom),
+        exact banned_litter.litter_dom L hL, }, },
+    { by_contradiction h',
+      simp only [near_litter_perm.is_exception, mem_litter_set, not_or_distrib, not_not, ha] at h,
+      obtain ⟨b, hb, rfl⟩ := hdiff (or.inr ⟨by rw [← hπL, h.2, smul_inv_smul, mem_litter_set], h'⟩),
+      refine h' ((w.atom_mem b hb L hL).mp _),
+      have := hπ.map_atom b (or.inl (or.inl hb)),
+      rw [w.complete_smul_atom_eq hb] at this,
+      rw [this, inv_smul_smul] at ha,
+      exact ha, }, },
+  { intro ha,
+    by_cases π⁻¹ • a ∈ w.atom_map.dom,
+    { rw w.atom_mem _ h L hL,
+      have := hπ.map_atom _ (or.inl (or.inl h)),
+      rw w.complete_smul_atom_eq h at this,
+      rw [this, smul_inv_smul],
+      exact ha, },
+    have haL : a ∈ litter_set ((w.litter_map L).get hL).fst,
+    { by_contradiction h',
+      obtain ⟨b, hb, rfl⟩ := hdiff (or.inl ⟨ha, h'⟩),
+      have := hπ.map_atom b (or.inl (or.inl hb)),
+      rw [w.complete_smul_atom_eq hb] at this,
+      rw [this, inv_smul_smul] at h,
+      exact h hb, },
+    by_contradiction h',
+    have : π.is_exception (π⁻¹ • a),
+    { left,
+      contrapose! h',
+      rw smul_inv_smul at h',
+      have := eq_of_mem_litter_set_of_mem_litter_set haL h',
+      rw [← hπL, smul_left_cancel_iff] at this,
+      exact this.symm, },
+    have : π.is_exception a,
+    { refine or.inr (λ h'', h' (h''.trans _)),
+      rw [inv_smul_eq_iff, hπL],
+      exact haL, },
+    obtain ((hdom | hdom) | hdom) := hπ.exception_mem a this,
+    { sorry, },
+    { sorry, },
+    { sorry, }, },
+end
+
+end weak_near_litter_approx
+
+end con_nf
